rpc/ServerSpec.v
@@ -5,13 +5,13 @@ Require Import libapplpi.
 Require Import Session.
 
 Inductive ServerSpec' : session -> proc -> Prop :=
-| SCall   : forall req res val,
-  ServerSpec' (Call req res) (OutAtom res val)
+| SCall   : forall req res x,
+  ServerSpec' (Call req res) (OutAtom res x)
 | SNotify : forall n,
   ServerSpec' (Notify n) zeroP.
 
-Inductive ServerSpec : proc -> Prop :=
-| SServer : forall b (ch : chan session b) P,
-  (forall msg, ServerSpec' msg (P msg)) ->
-  ServerSpec (ch ??* (fun msg => P msg)).
+Inductive ServerSpec : chan session true -> proc -> Prop :=
+| SServer : forall ch P,
+  (forall x, ServerSpec' x (P x)) ->
+  ServerSpec ch (ch ??* P).
 
