rpc/Progress.v
@@ -1,0 +1,16 @@
+Add LoadPath "../applpi".
+Add LoadPath "../proof".
+
+Require Import libapplpi.
+Require Import Session.
+Require Import ServerSpec ClientSpec.
+
+Inductive Progress : chan response true -> form -> Prop :=
+| progress : forall res x,
+  Progress res (OUTPUTS res x ISANY).
+
+Theorem rpc_progress : forall res S C f,
+  (forall ch, ServerSpec ch (S ch)) ->
+  (forall ch, ClientSpec ch res (C ch)) ->
+  Progress res f ->
+  (nilC # nuPl (fun c => parP (S c) (C c))) |=t (FMUSTEV (ALWAYS (STAT f))).
